Exitify done! 🎆
Here is the main theorem:

    Theorem exitifyProgram_WellScoped_JPV:
      forall pgm,
      WellScopedProgram pgm ->
      isJoinPointsValidProgram pgm ->
      WellScopedProgram (exitifyProgram pgm) /\
      isJoinPointsValidProgram (exitifyProgram pgm).

Of course, the are plenty of Admitted things in modules that this
depends on, e.g. JoinPointInvariants.v, VarSet.v, ScopeInvariant.v. But
all the stuff that relates to Exitification is proven.

examples/ghc/theories/JoinPointInvariants.v
@@ -307,6 +307,12 @@ Definition isjoinPointsAlt : CoreAlt -> VarSet -> bool :=
 
 Definition isJoinPointsValidPair := isJoinPointsValidPair_aux isJoinPointsValid isJoinRHS_aux.
 
+(* Top-level binders are never join-points *)
+Definition isJoinPointsValidProgram (pgm : CoreProgram)  :=
+  Forall (fun '(v,e) =>
+    isJoinId v = false /\
+    isJoinPointsValid e 0 emptyVarSet = true) (flattenBinds pgm).
+
 Lemma isJoinPointsValid_more_args:
   forall e n n' jps,
   n <= n' ->
